Add second implementation of parse function and a few tests for it

ParseTree.v
@@ -1,12 +1,21 @@
 Require Import Grammar.
 
+(* Type variable seems to be cluttering up the definitions below. *)
 Inductive parse_tree {A} :=
 | Leaf : A -> parse_tree
 | Node : A -> list parse_tree -> parse_tree.
-
 
 Definition getRoot (tree : parse_tree) : symbol :=
   match tree with
   | Node ntName _ => NT ntName
   | Leaf tName    => T tName
   end.
+
+Definition isNode {A} (tree : (@parse_tree A)) : bool :=
+  match tree with
+  | Node _ _ => true
+  | Leaf _   => false
+  end.
+
+Definition isLeaf {A} (tree : (@parse_tree A)) : bool :=
+  negb (isNode tree).
